FromNode constructor

xi-rope.dfy
@@ -25,38 +25,20 @@ module Rope {
       Content := [""];
     }
 
-
-    constructor FromNodes(nodes: seq<Rope>)
-      requires forall c: Rope :: c in nodes ==> c.Valid() && c.ValidLen()
-      requires |nodes| >= MIN_CHILDREN && |nodes| <= MAX_CHILDREN
-//      ensures Valid()
-//      ensures ValidLen()
-      modifies nodes
+    constructor FromNodes(left: Rope, right: Rope)
+      requires left.ValidNonRoot() && left.ValidLen() && right.ValidNonRoot() && right.ValidLen() && left.height == right.height && left.len == left.Len() && right.len == right.Len()
+      ensures Valid()
+      ensures ValidLen()
     {
-      var i := 0;
-      Content := [];
-      Repr := {};
-      var totalLen := 0;
-      val := InternalNode(nodes);
+      Repr := left.Repr + right.Repr + {this};
+      val := InternalNode([left, right]);
+      height := left.height + 1;
+      len := left.len + right.len;
+      Content := left.Content + right.Content;
 
-      while i < |nodes|
-      {
-        totalLen := totalLen + nodes[i].len;
-        Content := Content + nodes[i].Content;
-        var c := new Rope.Init();
-        c.len := nodes[i].len;
-        c.Content := nodes[i].Content;
-        c.Repr := c.Repr + nodes[i].Repr - {nodes[i]};
-        Repr := Repr + nodes[i].Repr;
-
-        i := i + 1;
-      }
-
-      len := totalLen;
-      Repr := Repr + {this};
     }
 
-    function ContentLen(c: seq<string>): int
+    function method ContentLen(c: seq<string>): int
       decreases |c|
     {
       if |c| == 0 then 0
@@ -79,7 +61,7 @@ module Rope {
     {
       match this.val
       case Leaf(v) => this.len == |v| && ContentLen(this.Content) == |v| && |Content| == 1
-      case InternalNode(children) => this.len == this.Len() && this.len >= 0 && forall c: Rope :: c in children ==> c.len <= this.len && c.ValidLen()
+      case InternalNode(children) => this.len >= 0 && forall c: Rope :: c in children ==> c.len <= this.len && c.ValidLen()
     }
 
     predicate ValidNonRoot()
@@ -95,13 +77,13 @@ module Rope {
           height >= 0 &&
           |children| >= MIN_CHILDREN &&
           |children| <= MAX_CHILDREN &&
-          forall c: Rope :: c in children ==> 
+          forall c: Rope :: c in children ==>
             c in Repr && this !in c.Repr && c.Repr < Repr && c.ValidNonRoot() &&
-            c.height == height - 1 && c.Content <= Content &&
+            c.height == height - 1 && |c.Content| <= |Content| &&
             forall cont: string :: cont in c.Content ==> cont in this.Content
       )
     }
-    
+
     predicate Valid()
       reads this, Repr
       requires MAX_LEAF_LEN >= MIN_LEAF_LEN
@@ -115,9 +97,9 @@ module Rope {
           height >= 0 &&
           |children| >= 2 &&
           |children| <= MAX_CHILDREN &&
-          forall c: Rope :: c in children ==> 
+          forall c: Rope :: c in children ==>
             c in Repr && this !in c.Repr && c.Repr < Repr &&
-            c.ValidNonRoot() && c.height == height - 1 && c.Content <= Content &&
+            c.ValidNonRoot() && c.height == height - 1 && |c.Content| <= |Content| &&
             forall cont: string :: cont in c.Content ==> cont in this.Content
       )
     }
@@ -203,139 +185,6 @@ module Rope {
 
               slice := finalSlice;
           }
-    }
-  }
-}
-
-
-
------------------
-
-
-module Rope {
-  const MAX_CHILDREN: nat := 4
-  const MIN_CHILDREN: nat := 2
-  const MAX_LEAF_LEN: nat := 10
-  const MIN_LEAF_LEN: nat := 2   // minimum size requirement when splitting
-
-  datatype Node = Leaf(value: string) | InternalNode(children: array<Rope>)
-
-  class Rope {
-    ghost var Repr: set<Rope>
-    ghost var Content: seq<string>
-
-    var val: Node
-    var len: int
-    var height: int
-
-    constructor Init()
-//      ensures Valid()
-//      ensures ValidLen()
-    {
-      val := Leaf("");
-      len := 0;
-      height := 0;
-      Repr := {this};
-      Content := [""];
-    }
-
-
-    constructor FromNodes(nodes: array<Rope>)
-//      requires forall c: Rope :: c in nodes ==> c.Valid() && c.ValidLen()
-     // requires |nodes| >= MIN_CHILDREN && |nodes| <= MAX_CHILDREN
-      
-      //ensures Valid()
-      //ensures ValidLen()
-      modifies nodes
-    {
-      var i := 0;
-      Content := [];
-      Repr := {};
-      var totalLen := 0;
-      var r := new Rope.Init();
-      var tmp := new Rope[nodes.Length](_ => r);
-      
-      while i < nodes.Length
-      {
-        tmp[i] := nodes[i];
-        totalLen := totalLen + tmp[i].len;
-        Content := Content + tmp[i].Content;
-        Repr := Repr + tmp[i].Repr;
-
-        i := i + 1;
-      }
-
-      val := InternalNode(tmp);
-      len := totalLen;
-      Repr := Repr + {this};
-    }
-  
-
-    function ContentLen(c: seq<string>): int
-      decreases |c|
-    {
-      if |c| == 0 then 0
-      else |c[0]| + ContentLen(c[1..])
-    }
-
-    function Len(): int
-      requires Valid()
-      reads *
-      decreases Repr
-    {
-      match this.val
-      case Leaf(v) => |v|
-      case InternalNode(children) => ContentLen(this.Content)
-    }
-
-    predicate ValidLen()
-      requires Valid()
-      reads *
-      decreases Repr
-    {
-      match this.val
-      case Leaf(v) => this.len == |v| && ContentLen(this.Content) == |v| && |Content| == 1
-      case InternalNode(children) => this.len == this.Len() && this.len >= 0 && forall k: int :: 0 <= k < children.Length ==> children[k].len <= this.len && children[k].ValidLen()
-    }
-
-    predicate ValidNonRoot()
-      reads *
-      requires MAX_LEAF_LEN >= MIN_LEAF_LEN
-      requires MIN_CHILDREN <= MAX_CHILDREN && MIN_CHILDREN >= 2
-      decreases Repr
-    {
-      this in Repr &&
-      (
-        match this.val
-        case Leaf(v) => |v| <= MAX_LEAF_LEN && Content == [v] && height == 0
-        case InternalNode(children) =>
-          height >= 0 &&
-          children.Length >= MIN_CHILDREN &&
-          children.Length <= MAX_CHILDREN &&
-          forall k: int :: 0 <= k < children.Length ==>
-            children[k] in Repr && this !in children[k].Repr && children[k].Repr < Repr && children[k].ValidNonRoot() &&
-            children[k].height == height - 1 && children[k].Content <= Content &&
-            forall cont: string :: cont in children[k].Content ==> cont in this.Content
-      )
-    }
-    
-    predicate Valid()
-      reads *
-      requires MAX_LEAF_LEN >= MIN_LEAF_LEN
-      requires MIN_CHILDREN <= MAX_CHILDREN && MIN_CHILDREN >= 2
-    {
-      this in Repr &&
-      (
-        match this.val
-        case Leaf(v) => |v| <= MAX_LEAF_LEN && Content == [v] && height == 0
-        case InternalNode(children) =>
-          height >= 0 &&
-          children.Length <= MAX_CHILDREN &&
-          forall k: int :: 0 <= k < children.Length ==>
-            children[k] in Repr && this !in children[k].Repr && children[k].Repr < Repr && children[k].ValidNonRoot() &&
-            children[k].height == height - 1 && children[k].Content <= Content &&
-            forall cont: string :: cont in children[k].Content ==> cont in this.Content
-      )
     }
   }
 }
